theories/Syntax/All.v
@@ -1,0 +1,2 @@
+From LogRel Require Export AutoSubst.Extra.
+From LogRel.Syntax Require Export Context Notations NormalForms Weakening UntypedReduction.
