theories/TypingProperties/DeclarativeProperties.v
@@ -1,7 +1,6 @@
-(** * LogRel.DeclarativeInstance: proof that declarative typing is an instance of generic typing. *)
+(** * LogRel.DeclarativeProperties: basic properties of declarative typing, showing it is an instance of generic typing. *)
 From Coq Require Import CRelationClasses.
-From LogRel.AutoSubst Require Import core unscoped Ast Extra.
-From LogRel Require Import Utils BasicAst Notations Context NormalForms UntypedReduction Weakening GenericTyping DeclarativeTyping.
+From LogRel Require Import Utils Syntax.All GenericTyping DeclarativeTyping.
 
 Import DeclarativeTypingData.
 
